semantics/evaluateScript.sml
@@ -188,6 +188,11 @@ Definition evaluate_def[nocompute]:
   ∧
   evaluate st env [Lannot e l] = evaluate st env [e]
   ∧
+  evaluate st env [Open path e] =
+    (case open_dec_env path env of
+       NONE => (st,Rerr (Rabort Rtype_error))
+     | SOME opened => evaluate st (extend_dec_env opened env) [e])
+  ∧
   evaluate_match st env v [] err_v = (st,Rerr (Rraise err_v))
   ∧
   evaluate_match st env v ((p,e)::pes) err_v =
@@ -208,9 +213,11 @@ Definition evaluate_def[nocompute]:
             (st2,r) => (st2,combine_dec_result env1 r))
      | (st1,Rerr v7) => (st1,Rerr v7))
   ∧
+  (* Check constructor applications in their lexical scope, even in bodies
+     that this declaration does not evaluate. *)
   evaluate_decs st env [Dlet locs p e] =
     (if ALL_DISTINCT (pat_bindings p) ∧
-        every_exp (one_con_check env.c) e
+        check_exp_constructors env.c e
      then
        case evaluate st env [e] of
          (st',Rval v) =>
@@ -226,7 +233,7 @@ Definition evaluate_def[nocompute]:
   evaluate_decs st env [Dletrec locs funs] =
     (st,
      if ALL_DISTINCT (MAP (λ(x,y,z). x) funs) ∧
-        EVERY (λ(f,n,e). every_exp (one_con_check env.c) e) funs
+        EVERY (λ(f,n,e). check_exp_constructors env.c e) funs
      then
        Rval <|v := build_rec_env funs env nsEmpty; c := nsEmpty|>
      else Rerr (Rabort Rtype_error))
@@ -251,6 +258,11 @@ Definition evaluate_def[nocompute]:
      Rval
        <|v := nsEmpty;
          c := nsSing cn (LENGTH ts,ExnStamp st.next_exn_stamp)|>)
+  ∧
+  evaluate_decs st env [Dopen locs path] =
+    (case open_dec_env path env of
+       NONE => (st,Rerr (Rabort Rtype_error))
+     | SOME opened => (st,Rval opened))
   ∧
   evaluate_decs st env [Dmod mn ds] =
     (case evaluate_decs st env ds of
@@ -360,4 +372,3 @@ Theorem evaluate_decs_ind =
   |> Q.SPECL [‘λv1 v2 v3. T’,‘λv1 v2 v3 v4 v5. T’,‘P’]
   |> SIMP_RULE std_ss []
   |> Q.GEN ‘P’;
-
